proofs/printing/lval_notations.v
@@ -1,128 +1,115 @@
-From Coq Require Import ZArith.
+Set Implicit Arguments.
+Unset Strict Implicit.
+Unset Printing Implicit Defensive.
+
+From Stdlib Require Import ZArith.
 From mathcomp Require Import ssreflect ssrbool ssrfun ssrnat eqtype seq.
 
 Require Import expr.
 Require Import expr_notations.
 
-(** * Display notations for Jasmin left values
+(* TODO Add a docstring at the top of the file with every notation explained.
+Give an exhaustive list of all the cases that are not supported by notations.
+Here's the previous one as inspiration (needs updating):
 
-    Wrap a [lval] in [lval:( lv )] to view it in Jasmin-like syntax.
-    Example:
-      Check lval:( aset[U64](x, #0) ).
 
-    Notation summary:
-      - lnone[b]             = discard of type bool   (Lnone _ abool)
-      - lnone[i]             = discard of type int    (Lnone _ aint)
-      - lnone[ws]            = discard of type word   (Lnone _ (aword ws))
-      - lnone[ws, len]       = discard of type array  (Lnone _ (aarr ws len))
-      - x                    = variable (Lvar)
-      - st[w](e)         = unaligned memory write of word size w to address e
-      - aset[w](v, e)         = aligned array element write at index e
-      - asub[w](v, len, e)    = aligned subarray write of word size w
+-(** * Display notations for Jasmin left values
+-
+-    Wrap a [lval] in [lval:( lv )] to view it in Jasmin-like syntax.
+-    Example:
+-      Check lval:( aset[U64](x, #0) ).
+-
+-    Notation summary:
+-      - lnone[b]             = discard of type bool   (Lnone _ abool)
+-      - lnone[i]             = discard of type int    (Lnone _ aint)
+-      - lnone[ws]            = discard of type word   (Lnone _ (aword ws))
+-      - lnone[ws, len]       = discard of type array  (Lnone _ (aarr ws len))
+-      - x                    = variable (Lvar)
+-      - mem[w](e)         = unaligned memory write of word size w to address e
+-      - aset[w](v, e)         = aligned array element write at index e
+-      - asub[w](v, len, e)    = aligned subarray write of word size w
+-
+-    Not supported:
+-      - [Lmem Aligned w vi e]  : aligned memory write (only [Lmem Unaligned]
+-                                 is covered via [mem[w](e)])
+-      - [Laset] with alignment other than [Aligned] or scale other than
+-        [AAscale]
+-      - [Lasub] with scale other than [AAscale]
+-
+-    Precedence: all constructors are atoms (level 0).
+-*)
 
-    Not supported:
-      - [Lmem Aligned w vi e]  : aligned memory write (only [Lmem Unaligned]
-                                 is covered via [st[w](e)])
-      - [Laset] with alignment other than [Aligned] or scale other than
-        [AAscale]
-      - [Lasub] with scale other than [AAscale]
+ *)
 
-    Precedence: all constructors are atoms (level 0).
-*)
+(* Bridge coercion: bare gvar in lval position elaborates to Lvar v.(gv) *)
+Definition lvar_of_gvar (v : gvar) : lval := Lvar v.(gv).
+Coercion lvar_of_gvar : gvar >-> lval.
 
-Declare Custom Entry lval.
-
-(* -------------------------------------------------------------------------- *)
-(* Entry and exit *)
-
-Notation "lval:( e )" := e
-  (e custom lval at level 99,
-   format "'lval:(' e ')'").
-
-Notation "rocq:( e )" := e
-  (in custom lval at level 0, e constr at level 99).
-
-Notation "( e )" := e
-  (in custom lval at level 0, e custom lval at level 99).
-
-(* -------------------------------------------------------------------------- *)
-(* Discard *)
+Declare Scope jlval_scope.
+Delimit Scope jlval_scope with L.
+Bind Scope jlval_scope with lval.
 
 Notation "lnone[ 'b' ]" := (Lnone dummy_var_info abool)
-  (in custom lval at level 0).
+  (at level 0) : jlval_scope.
 Notation "lnone[ 'i' ]" := (Lnone dummy_var_info aint)
-  (in custom lval at level 0).
+  (at level 0) : jlval_scope.
 Notation "lnone[ ws ]" := (Lnone dummy_var_info (aword ws))
-  (in custom lval at level 0, ws constr at level 0).
+  (at level 0, ws constr at level 0) : jlval_scope.
 Notation "lnone[ ws , len ]" := (Lnone dummy_var_info (aarr ws len))
-  (in custom lval at level 0, ws constr at level 0, len constr at level 0).
+  (at level 0, ws constr at level 0, len constr at level 0)
+  : jlval_scope.
 
-(* -------------------------------------------------------------------------- *)
-(* Variable *)
+Notation "mem[ w ]( e )" := (Lmem Unaligned w dummy_var_info e%E)
+  (at level 0, w constr at level 0, e at level 99) : jlval_scope.
 
-Notation "x" := (Lvar x.(gv))
-  (in custom lval at level 0, x constr at level 0).
+Notation "aset[ w ]( v , i )" :=
+  (Laset Aligned AAscale w v.(gv) i%E)
+  (at level 0, w constr at level 0, v constr at level 0,
+   i at level 99) : jlval_scope.
 
-(* -------------------------------------------------------------------------- *)
-(* Aligned memory store --st[w](e) *)
-
-Notation "st[ w ]( e )" := (Lmem Unaligned w dummy_var_info e)
-  (in custom lval,
-   w constr at level 0, e custom expr at level 0).
-
-(* -------------------------------------------------------------------------- *)
-(* Aligned array element write --aset[w](v, i) *)
-
-Notation "aset[ w ]( v , i )" := (Laset Aligned AAscale w v.(gv) i)
-  (in custom lval,
-   w constr at level 0, v constr at level 0, i custom expr at level 99).
-
-(* -------------------------------------------------------------------------- *)
-(* Aligned subarray write --asub[w](v, len, i) *)
-
-Notation "asub[ w ]( v , len , i )" := (Lasub AAscale w len v.(gv) i)
-  (in custom lval,
-   w constr at level 0, v constr at level 0, len constr at level 0,
-   i custom expr at level 99).
+Notation "asub[ w ]( v , len , i )" :=
+  (Lasub AAscale w len v.(gv) i%E)
+  (at level 0, w constr at level 0, v constr at level 0,
+   len constr at level 0, i at level 99) : jlval_scope.
 
 Section LvalTests.
 
 Context (x y : gvar) (gx gy : gvar).
 
-Goal lval:( lnone[b] ) = Lnone dummy_var_info abool. done. Qed.
-Goal lval:( lnone[i] ) = Lnone dummy_var_info aint. done. Qed.
-Goal lval:( lnone[U64] ) = Lnone dummy_var_info (aword U64). done. Qed.
-Goal lval:( lnone[U32] ) = Lnone dummy_var_info (aword U32). done. Qed.
-Goal lval:( lnone[U64, 4] ) = Lnone dummy_var_info (aarr U64 4). done. Qed.
-Goal lval:( x ) = Lvar x.(gv). done. Qed.
+Goal (lnone[b])%L = Lnone dummy_var_info abool. done. Qed.
+Goal (lnone[i])%L = Lnone dummy_var_info aint. done. Qed.
+Goal (lnone[U64])%L = Lnone dummy_var_info (aword U64). done. Qed.
+Goal (lnone[U32])%L = Lnone dummy_var_info (aword U32). done. Qed.
+Goal (lnone[U64, 4])%L = Lnone dummy_var_info (aarr U64 4). done. Qed.
+Goal (x : lval) = Lvar x.(gv). done. Qed.
 
-Goal lval:( st[U64](#0) ) =
+Goal (mem[U64](0))%L =
   Lmem Unaligned U64 dummy_var_info (Pconst 0). done. Qed.
-Goal lval:( st[U32](#0) ) =
+Goal (mem[U32](0))%L =
   Lmem Unaligned U32 dummy_var_info (Pconst 0). done. Qed.
-Goal lval:( st[U64](gx) ) =
+Goal (mem[U64](gx))%L =
   Lmem Unaligned U64 dummy_var_info (Pvar gx). done. Qed.
-Goal lval:( st[U64](gx +64u #4) ) =
+Goal (mem[U64](gx +64u 4))%L =
   Lmem Unaligned U64 dummy_var_info
     (Papp2 (Oadd (Op_w U64)) (Pvar gx) (Pconst 4)).
 done. Qed.
 
-Goal lval:( aset[U64](x, #0) ) =
+Goal (aset[U64](x, 0))%L =
   Laset Aligned AAscale U64 x.(gv) (Pconst 0). done. Qed.
-Goal lval:( aset[U32](x, #0) ) =
+Goal (aset[U32](x, 0))%L =
   Laset Aligned AAscale U32 x.(gv) (Pconst 0). done. Qed.
-Goal lval:( aset[U64](x, gx) ) =
+Goal (aset[U64](x, gx))%L =
   Laset Aligned AAscale U64 x.(gv) (Pvar gx). done. Qed.
-Goal lval:( aset[U64](x, gx +64u #1) ) =
+Goal (aset[U64](x, gx +64u 1))%L =
   Laset Aligned AAscale U64 x.(gv)
     (Papp2 (Oadd (Op_w U64)) (Pvar gx) (Pconst 1)).
 done. Qed.
 
-Goal lval:( asub[U64](x, 4, #0) ) =
+Goal (asub[U64](x, 4, 0))%L =
   Lasub AAscale U64 4 x.(gv) (Pconst 0). done. Qed.
-Goal lval:( asub[U32](x, 8, #0) ) =
+Goal (asub[U32](x, 8, 0))%L =
   Lasub AAscale U32 8 x.(gv) (Pconst 0). done. Qed.
-Goal lval:( asub[U64](x, 4, gx) ) =
+Goal (asub[U64](x, 4, gx))%L =
   Lasub AAscale U64 4 x.(gv) (Pvar gx). done. Qed.
 
 End LvalTests.
