proofs/printing/syntax.v
@@ -3,27 +3,26 @@ From Coq Require Import ZArith.
 
 Require Import expr.
 
+(* -------------------------------------------------------------------------- *)
+(* Lightweight notations for printing. *)
+
 Notation mki i := (MkI dummy_instr_info i) (only parsing).
 
 Notation cassgn lv ty e := (mki (Cassgn lv AT_none ty e)) (only parsing).
 
-Notation copn lvs o es :=
-  (mki (Copn lvs AT_none o es)) (only parsing).
+Notation copn lvs o es := (mki (Copn lvs AT_none o es)) (only parsing).
 
 Notation crandombytes lv ws n e :=
-  (mki (Csyscall [:: lv] (RandomBytes ws n) [:: e])) (only parsing).
+  (mki (Csyscall [:: lv] (RandomBytes ws n) [:: e]))
+  (only parsing).
 
-Notation cassert l e :=
-  (mki (Cassert (l%string, e))) (only parsing).
+Notation cassert l e := (mki (Cassert (l%string, e))) (only parsing).
 
-Notation cif e c1 c2 :=
-  (mki (Cif e c1 c2)) (only parsing).
+Notation cif e c1 c2 := (mki (Cif e c1 c2)) (only parsing).
 
-Notation cfor v r c :=
-  (mki (Cfor v r c)) (only parsing).
+Notation cfor v r c := (mki (Cfor v r c)) (only parsing).
 
-Notation cwhile c1 e c2 :=
-  (mki (Cwhile Align c1 e dummy_instr_info c2)) (only parsing).
+Notation cwhile c1 e c2 := (mki (Cwhile Align c1 e dummy_instr_info c2))
+  (only parsing).
 
-Notation ccall lvs f es :=
-  (mki (Ccall lvs f es)) (only parsing).
+Notation ccall lvs f es := (mki (Ccall lvs f es)) (only parsing).
